NI done

NI.v
@@ -1,31 +1,69 @@
 From TL Require Import Identifier Environment Imperative Types Augmented Bridge.
 From TL Require Import WellFormedness LowEq. 
 From TL Require Import NIBridge.
-From TL Require Import InductionPrinciple.
+From TL Require Import Adequacy.
+From TL.lib Require Import InductionPrinciple.
+From Coq Require Import Lia.
+Require Import Coq.Program.Equality.
 
-Lemma TINI_idx:
-  forall Γ c st1 st2 st1_end st2_end n1 n2 pc,
+Definition TINI_idx (n1: nat): Prop :=
+  forall Γ c st1 st1_end st2 st2_end pc n2,
     -{ Γ, pc ⊢ c }- ->
     state_low_eq Γ st1 st2 ->
-    multistep_idx 〈 c, st1 〉 〈 STOP, st1_end 〉 n1 ->
-    multistep_idx 〈 c, st2 〉 〈 STOP, st2_end 〉 n2 ->
+    multistep_idx 〈c, st1 〉 〈STOP, st1_end 〉 n1 ->
+    multistep_idx 〈c, st2 〉 〈STOP, st2_end 〉 n2 ->
     state_low_eq Γ st1_end st2_end.
-Proof.
-  intros Γ c st1 st2 st1_end st2_end n1 n2 pc H_wt H_leq H_st1 H_st2.
-  
-  revert Γ c st1 st2 H_wt H_leq H_st1 H_st2.
 
+Lemma tini_idx: forall n1, TINI_idx n1.
+Proof.
   apply strongind.
-  - intros. inversion H_st1. inversion H_st2.
-    + subst. apply H_leq.
-    + subst. inversion H0.
-  - intros.
-    inversion H_st1; subst.  
-    inversion H_st2.
-    + subst. inversion H0.
-    + subst.
-      destruct y as [c1 st1'].
-      destruct y0 as [c2 st2'].
+  {
+    unfold TINI_idx. intros. 
+    inversion H1; subst; inversion H2; subst; 
+    auto; inversion H3.
+  }
+  {
+    unfold TINI_idx.
+    intros.
+    inversion H1.
+    specialize (bridge_adequacy (S n) c st1 st1_end H2 Γ pc H0 H4) as [H_adeq_st11 | H_adeq_st12]; inversion H2; subst.
+    + inversion H11.
+    + specialize (bridge_adequacy n2 c st2 st2_end H3 Γ pc H0 H5) as [H_adeq_st21 | H_adeq_st22]. subst.
+      * inversion H11.
+      * destruct H_adeq_st12 as [ev1 [n1' [cfg1' [k1 [H_bridge1 [H_multistep1 H_index1]]]]]].
+        destruct H_adeq_st22 as [ev2 [n2' [cfg2' [k2 [H_bridge2 [H_multistep2 H_index2]]]]]].
+
+        destruct cfg1' as [c1 st1'].
+        destruct cfg2' as [c2 st2'].
+
+        specialize (ni_bridge_num Γ pc c H0 c1 c2 st1 st2 ev1 ev2 st1' st2' n1' n2' H1 H_bridge1 H_bridge2) as [H_leq' [H_c_eq [H_low_event_eq H_event_eq]]].
+        subst.
+
+        assert (k1 <= n) as H_k1 by lia.
+        (* specialize (H k1 H_k1 Γ c2 st1' st1_end st2' st2_end pc k2 H0 H_leq' H_index1 H_index2) as H_ret. *)
+
+        specialize (preservation_wf_bridge Γ pc c c2 st2 st2' ev2 n2' H0 H_bridge2 H5) as [H_wf_mem' H_wf_cmd'].
+
+         destruct (eq_cmd_stop_dec c2) as [Heq | Hneq].
+         {
+            subst. 
+            assert (st1' = st1_end). 
+            {
+              apply multi_idx_start_with_stop_states_unchanged with (n:=k1) (c:=STOP) in H_multistep1 as [_ H_st1_eq].
+              assumption.
+            }
+            assert (st2' = st2_end). 
+            {
+              apply multi_idx_start_with_stop_states_unchanged with (n:=k2) (c:=STOP) in H_multistep2 as [_ H_st2_eq].
+              assumption.
+            }
+            subst. assumption.
+         }
+         {
+            apply H with (m:=k1) (c:=c2) (st1:=st1') (st2:=st2') (pc:=pc) (n2:=k2);auto.
+         }
+  }
+Qed.
    
 Theorem TINI:
   forall Γ c st1 st2 st1_end st2_end pc,
