Adequacy.v
@@ -1,0 +1,24 @@
+From TL Require Import Identifier Environment Imperative Types Augmented WellFormedness Bridge.
+
+Lemma adequacy_of_event_steps:
+  forall Γ pc c m cfg',
+    wf_mem m Γ ->
+    -{ Γ, pc ⊢ c }- ->
+    〈c, m 〉 ⇒ cfg' ->
+    exists ev, event_step Γ ev 〈c, m 〉 cfg'.
+Proof.
+Admitted.
+
+Theorem bridge_adequacy:
+  forall n c m m_end,
+    multistep_idx 〈c, m 〉 〈STOP, m_end 〉 n ->
+    forall Γ pc, 
+      -{ Γ, pc ⊢ c }-  ->
+      wf_mem m Γ  ->
+      (c = STOP \/
+        exists ev n' cfg' k,
+          (〈 c, m 〉 ↷ (Γ, ev, n') cfg') /\
+          multistep_idx cfg' 〈STOP, m_end 〉 k /\ k < n).
+
+Proof.
+Admitted.
